\ifdefined\mainprogram{}
\else
\include{head}
\fi

\begin{align}
	\as &= \frac{g^2}{(4\pi)^2}
	\\
	v^{\iota\alpha\beta\gamma}
	&=\left(2\metric^{\iota\beta}\metric^{\alpha\gamma}
	-\metric^{\iota\alpha}\metric^{\beta\gamma}-
	2\metric^{\iota\gamma}\metric^{\alpha\beta}\right)
\end{align}
d dim integrals from P$\&$S

\begin{align}
\int \frac{\dx ^d l}{(2\pi)^d} \frac{1}{\left(l^2-\Delta\right)^n} 
&=
\frac{(-1)^n\imag}{(4\pi)^{d/2}} \frac{\Gamma\left(n-\frac{d}{2}\right)}{\Gamma(n)}\left(\frac{1}{\Delta}\right)^{n-\frac{d}{2}}
\\
\int \frac{\dx ^d l}{(2\pi)^d} \frac{l^2}{\left(l^2-\Delta\right)^n} 
&=
\frac{(-1)^{n-1}\imag}{(4\pi)^{d/2}}\frac{d}{2} \frac{\Gamma\left(n-\frac{d}{2}-1\right)}{\Gamma(n)}\left(\frac{1}{\Delta}\right)^{n-\frac{d}{2}-1}
\\
\int \frac{\dx ^d l}{(2\pi)^d} \frac{l^	\mu l^\nu}{\left(l^2-\Delta\right)^n} 
&=
\frac{(-1)^{n-1}\imag}{(4\pi)^{d/2}}\frac{\metric^{\mu \nu}}{2} \frac{\Gamma\left(n-\frac{d}{2}-1\right)}{\Gamma(n)}\left(\frac{1}{\Delta}\right)^{n-\frac{d}{2}-1}
\end{align}

Crucial formulae:

\begin{align}
\frac{1}{A_1^{m_1}...A_n^{m_n}} 
&= \int_{0}^{1} \dx x_1 \dots \dx x_n \delta\left(\sum x_i -1\right) \frac{\prod x_i^{m_i-1}}{\left(\sum x_iA_i\right)^{\sum m_i}}\frac{\Gamma\left(\sum m_i\right)}{\prod \Gamma(m_i)}
\label{denominatorproductAsIntegral}
\\
\contraction{}{\psi}{(x)}{\overline{\psi}}\psi (x) \overline \psi (0) 
&=
\gf(x)= \frac{\imag \slashed{x}}{2\pi^2x^4}
= \frac{\imag \Gamma\left({\frac{d}{2}}\right) \slashed{x}}{2\pi^2\left(x^2\right)^\frac{d}{2}}
\\
&=
\frac{\Gamma\left(\frac{D+1}{2}\right)}{2\pi^{\frac{D+1}{2}}}\frac{\imag \slashed x}{\left(-x^2+\imag \epsilon\right)^{\frac{D+1}{2}}}
\\
&=
\frac{\Gamma\left(\frac{d}{2}\right)}{2\pi^{\frac{d}{2}}}\frac{\imag \slashed x}{\left(-x^2+\imag \varepsilon\right)^{\frac{d}{2}}}
\\
CHECK: \contraction{}{A}{^{\mu,a}(x)}{\overline{A}} A^{\mu,a}(x)A^{\nu,b}(0) 
&= \frac{-\imag}{4 \pi^2} \frac{\metric^{\mu \nu}}{x^2} \text{(must be wrong)}
\\
&=
\frac{-\imag}{4 \pi^2} \frac{\Gamma\left(\frac{d}{2}-1\right)\metric^{\mu \nu}\delta^{ab}}{\left(x^2\right)^{\frac{d}{2}-1}} 
\\
&=
\frac{-\color{red}{1}}{4 \pi^{\frac{d}{2}}} \frac{\Gamma\left(\frac{d}{2}-1\right)\metric^{\mu \nu}\delta^{ab}}{\left(-x^2+\imag\epsilon\right)^{\frac{d}{2}-1}} 
\\
\slashed A &= A^\mu \gamma_\mu = A^{\mu,a} \gamma_\mu t^a
\\
t^a t^a &= C_2 \mathbb{1}  = C_F \mathbb{1}
\\
\slashed x \slashed x 
&= x^2
\\
\slashed a \slashed b \slashed a 
&=
- \slashed b a^2 +2 \skpt{a}{b}\slashed a
\\
\gamma_\mu \gamma^\nu \gamma^\mu 
&=
-(d-2)\gamma^\nu
\\
\gamma^\mu \gamma_\mu 
&=
d
\end{align}

work in gauges (q: quantum, c: classical fields)
\begin{align}
x_{\mu} A^{\mu,c} = 0
\\
\cov_\mu^{c} A^{\mu,q} = 0
\end{align}











\ifdefined\mainprogram{}
\else
\include{end}
\fi